\begin{gather*}
\infer[\mbox{Ax}]{\Gamma, \alpha \vdash \alpha}{}
~~~~ ~~~~
\infer[\mbox{EFQ}]{\Gamma \vdash \beta}{\Gamma \vdash \bot}
\\ \\ 
\infer[\wedge\mbox{-I}]{\Gamma_1, \Gamma_2 \vdash \alpha_1 \wedge \alpha_2}{
    \Gamma_1 \vdash \alpha_1
    &
    \Gamma_2 \vdash \alpha_2
}
~~~~ ~~~~
\infer[\wedge\mbox{-E}]{\Gamma \vdash \alpha_i}{
    \Gamma \vdash \alpha_1 \wedge \alpha_2
}
\\ \\ 
\infer[\vee\mbox{-I}]{\Gamma\vdash \alpha_1 \vee \alpha_2}{\Gamma \vdash \alpha_i}
~~~~ ~~~~
\infer[\vee\mbox{-E}]{\Gamma_1, \Gamma_2 \vdash \beta}{
    \Gamma_1 \vdash \alpha_1 \vee \alpha_2
    &
    \Gamma_2, \alpha_1 \vdash \beta
    &
    \Gamma_2, \alpha_2 \vdash \beta
}
\\ \\ 
\infer[\rightarrow\mbox{-I}]{\Gamma \vdash \alpha \rightarrow \beta}{\Gamma, \alpha \vdash \beta}
~~~~ ~~~~
\infer[\rightarrow\mbox{-E}]{\Gamma_1, \Gamma_2 \vdash \beta}{\Gamma_1 \vdash \alpha & \Gamma_2 \vdash \alpha \rightarrow \beta}
\end{gather*}