\begin{eqnarray*}
\pi_i(\v_1, \v_2) &\leadsto& \v_i\\
(\lambda x.\t_1)\v_2 &\leadsto& \t_1 [x \mapsto \v_2]\\
\mathtt{case}\ \ \mathtt{in}_i\v \ \ \mathtt{of}\ (\mathtt{in}_1\ x_1 \mapsto \t_1\  \lvert\  \mathtt{in}_2 \ x_2 \ \mapsto \t_2) &\leadsto& \t_i [x_i \mapsto \v]\\
\mathtt{let}\ ()=()\ \mathtt{in} \ \e &\leadsto& \e\\
\mathtt{let}\ (x_1,x_2)=(\e_1,\e_2)\ \mathtt{in}\ \e &\leadsto& \e[x \mapsto \e_1,x \mapsto \e_2]\\
(\lambda x.\e_1)\e_2 &\leadsto& \e_1[x \mapsto \e_2]\\
\mathtt{bind}\ x = \mathtt{return} \ \e_1\ \mathtt{in} \ \e_2\ &\leadsto&\ \e_2 [x \mapsto \e_1]\\
\mathtt{force}( \mathtt{suspend}\ \e)\ &\leadsto& \e\\
\mathtt{let}\  \floor{x}=\floor{\v}\  \mathtt{in}\ \e\ &\leadsto& \e[x\mapsto \v]\\
\mathtt{case}\ \ \mathtt{in}_i\e \ \ \mathtt{of}\ (\mathtt{in}_1\ x_1 \mapsto \e_1\  \lvert\  \mathtt{in}_2 \ x_2 \mapsto \e_2) &\leadsto& \e_i [x_i \mapsto \e]
\end{eqnarray*}